pv/Completeness.v
@@ -37,3 +37,69 @@ Proof.
   subst.
   repeat split; try tauto.
 Qed.
+
+
+
+Lemma completeness_of_protocol: 
+ forall (program: list ins)(CPU_trace rm_first_CPU_trace rm_last_CPU_trace: list CPU_state)
+  (first_CPU_state last_CPU_state: CPU_state)
+  (action_trace: list action_type)(memory_trace: list action_type),
+  CPU_trace = cons first_CPU_state rm_first_CPU_trace ->
+  CPU_trace = rm_last_CPU_trace ++ [last_CPU_state] ->
+  (exists (mem_list: list (int256 -> int256))(first_mem last_mem: int256 -> int256),
+  length mem_list = length action_trace /\
+  eval_ins_list program
+  (combine_to_pc_state first_CPU_state first_mem)
+  (combine_to_act_state_list rm_last_CPU_trace mem_list action_trace)
+  (combine_to_pc_state last_CPU_state last_mem))
+-> constraints program CPU_trace action_trace memory_trace.
+Proof.
+  intros.
+  destruct H1 as [mem_list [first_mem [last_mem [H1 H2]]]].
+  split.
+  remember (combine_to_pc_state first_CPU_state first_mem) as x.
+  remember (combine_to_act_state_list rm_last_CPU_trace mem_list action_trace) as y.
+  remember (combine_to_pc_state last_CPU_state last_mem) as z.
+  destruct H2 as [program].
+   + apply trace_CPU with (rm_first_CPU_trace:=rm_first_CPU_trace) (first_CPU_state:=first_CPU_state).
+    - tauto.
+    - unfold combine_to_pc_state in *.
+      unfold Definition_and_soundness.Build_pc_state  in *.
+      unfold Definition_and_soundness.Build_program_state in *.
+      rewrite Heqx in H2.
+      simpl in H2.
+      tauto.
+   -  unfold combine_to_pc_state in *.
+      unfold Definition_and_soundness.Build_pc_state  in *.
+      unfold Definition_and_soundness.Build_program_state in *.
+      rewrite Heqx in H4.
+      simpl in H4.
+      tauto.
+    - destruct H6 as[n ?].
+Admitted.
+
+(*      induction n.
+      * simpl in H6.
+        destruct H6.
+        inversion H6.
+        rewrite H8 in H5.
+        rewrite Heqx in H7.
+        rewrite Heqz in H7.
+        inversion H7.*)
+(*
+      rewrite H.
+      induction rm_first_CPU_trace.
+      * simpl.
+        pose proof adjacent_CPU_state_nil.
+        pose proof adjacent_CPU_state_cons.
+        specialize (H0 eval_constraint last_CPU_state).
+        tauto.
+      * pose proof adjacent_CPU_state_nil.
+        pose proof adjacent_CPU_state_cons.
+        pose proof cons_app_eq a rm_last_CPU_trace.
+        destruct H9 as [last_two_CPU_trace [rm_last_two_CPU_trace ?]].
+        rewrite H9.
+        specialize (H8 eval_constraint last_two_CPU_trace last_CPU_state rm_last_two_CPU_trace).
+        apply H8.
+subst.
+*)
