pv/Soundness.v
@@ -1,0 +1,1058 @@
+Require Import Coq.ZArith.ZArith.
+Require Import Coq.Strings.String.
+Require Import Coq.Vectors.Vector.
+Require Import Coq.Lists.List. Import ListNotations.
+Require Import Coq.Sorting.Permutation.
+Require Import Coq.Sets.Multiset.
+Require Import SetsClass.SetsClass. Import SetsNotation.
+Require Import compcert.lib.Integers.
+Require Import Coq.micromega.Lia.
+Require Import Coq.Logic.FunctionalExtensionality.
+Require Import Definition_and_soundness.  Import Definition_and_soundness.
+
+Local Open Scope string.
+Local Open Scope sets.
+Local Open Scope list.
+
+Import Int256.
+Import Lang.
+Import program_state.
+Import CPU_state.
+Import pc_state.
+Import act_state.
+
+Definition Build_program_state (memory: int256 -> int256) (stack: list int256): program_state :=
+  {| program_state.memory := memory; program_state.stack := stack |}.
+
+Definition Build_pc_state (pc: nat) (state: program_state): pc_state :=
+  {| pc_state.pc := pc; pc_state.state := state |}.
+
+Theorem soundness:
+  (* CPU_trace_list is without first and last CPU_state *)
+  forall (program: list ins)(CPU_trace rm_first_CPU_trace rm_last_CPU_trace: list CPU_state)
+  (first_CPU_state last_CPU_state: CPU_state)
+  (action_trace: list action_type)(memory_trace: list action_type),
+  constraints program CPU_trace action_trace memory_trace ->
+  CPU_trace = cons first_CPU_state rm_first_CPU_trace ->
+  CPU_trace = rm_last_CPU_trace ++ [last_CPU_state] ->
+  exists (mem_list: list (int256 -> int256))(first_mem last_mem: int256 -> int256),
+  length mem_list = length action_trace /\
+  eval_ins_list program
+  (combine_to_pc_state first_CPU_state first_mem)
+  (combine_to_act_state_list rm_last_CPU_trace mem_list action_trace)
+  (combine_to_pc_state last_CPU_state last_mem) /\
+  (forall address: int256, last_mem_prop last_mem memory_trace address)
+  .
+Proof.
+  intros program CPU_trace rm_first_CPU_trace rm_last_CPU_trace first_CPU_state last_CPU_state action_trace memory_trace.
+  revert program CPU_trace rm_first_CPU_trace rm_last_CPU_trace first_CPU_state last_CPU_state memory_trace.
+  apply rev_ind with (l := action_trace).
+  - intros. subst. inversion H. subst.
+    inversion H0. subst.
+    inversion H8. symmetry in H13, H14. subst. clear H8.
+    (* CPU_trace should be a single value list; adjacent_CPU_state_for_action_trace has two constructors *)
+    inversion H4. subst. inversion H8; subst.
+    + symmetry in H1. apply app_eq_unit in H1. inversion H1. clear H1.
+      { inversion H12. clear H12. subst. inversion H13. subst. clear H13.
+        unfold combine_to_act_state_list. exists nil. simpl. (* mem_list = [] *)
+        exists (fun _ => Int256.zero). exists (fun _ => Int256.zero). (* first_mem = last_mem = fun (n: int256) => Int256.zero *)
+        destruct program.
+        - inversion H2. subst. simpl in H1. inversion H1. contradiction. (* program = [] *)
+        - intros.
+          split.
+          + tauto.
+          + split.
+            * apply sigma; try auto; try apply ActionListNil.
+              unfold combine_to_pc_state, Build_pc_state, Build_program_state; simpl; exists 0; simpl.
+              sets_unfold.
+              tauto.
+            * intros.
+              assert (memory_trace = []).
+              {
+                inversion H5; subst.
+                simpl in H1.
+                apply Permutation_nil.
+                tauto.
+              }
+              rewrite H1.
+              apply not_in_memory_trace.
+              simpl.
+              intros.
+              contradiction.
+              tauto.
+      }
+      { inversion H12. discriminate. }
+    + apply app_eq_nil in H13. inversion H13. discriminate.
+  - intros. subst. inversion H0. subst. rewrite H2 in H0, H1, H3, H5, H8.
+    assert (action_trace_constraint rm_last_CPU_trace l).
+    {
+      apply trace_action.
+      inversion H5. subst.
+      inversion H9.
+      - symmetry in H12.
+        apply app_eq_nil in H12.
+        inversion H12.
+        discriminate.
+      - apply app_inj_tail in H10.
+        destruct H10.
+        apply app_inj_tail in H11.
+        destruct H11.
+        rewrite H10 in H13.
+        rewrite H11 in H13.
+        apply H13.
+    }
+    assert (CPU_trace_constraint rm_last_CPU_trace).
+    {
+      inversion H1. subst.
+      rewrite <- H2 in H10.
+      inversion H10.
+      clear H10.
+      rewrite <- H15 in H11.
+      rewrite <- H15 in H12.
+      clear rm_first_CPU_trace0 first_CPU_state0 H15 H16.
+      inversion H13; subst.
+      - symmetry in H14.
+        apply app_eq_unit in H14.
+        inversion H14.
+        + inversion H10.
+          apply action_CPU_trace_len_cons in H9.
+          rewrite H15 in H9.
+          discriminate.
+        + inversion H10.
+          discriminate.
+      - assert (l0 ++ [x0; y]= (l0 ++ [x0]) ++ [y]). { rewrite <- app_assoc. tauto. }
+        rewrite H16 in H10.
+        apply app_inj_tail in H10.
+        inversion H10.
+        destruct rm_last_CPU_trace.
+        + apply app_eq_nil in H17.
+          inversion H17.
+          discriminate.
+        + rewrite H17 in H15.
+          rewrite <- app_comm_cons in H2.
+          inversion H2.
+          rewrite <- H20.
+          pose proof (trace_CPU (first_CPU_state :: rm_last_CPU_trace) rm_last_CPU_trace first_CPU_state).
+          apply H19.
+          tauto.
+          tauto.
+          tauto.
+          rewrite <- H20 in H15.
+          tauto.
+    }
+    assert (multiset_constraint rm_last_CPU_trace program).
+    { 
+      inversion H3.
+      rewrite map_app in H11.
+      apply Forall_app in H11.
+      inversion H11.
+      apply trace_multiset.
+      tauto.
+    }
+    assert (action_trace_timestamp_constraint l).
+    {
+      inversion H4.
+      - symmetry in H13.
+        apply app_eq_nil in H13.
+        inversion H13.
+        discriminate.
+      - symmetry in H12.
+        apply app_eq_unit in H12.
+        inversion H12.
+        + inversion H14.
+          rewrite H15.
+          apply ActionListTraceNil.
+        + inversion H14.
+          discriminate.
+      - apply app_inj_tail in H12.
+        inversion H12.
+        rewrite <- H15.
+        apply H14.
+    }
+    assert (exists memory_trace', memory_trace_legal l memory_trace' /\
+    (x.(mem_ins) <> non /\ (exists l1' l2', (memory_trace' = l1' ++ l2' /\ memory_trace = l1' ++ [x] ++ l2')) \/
+    (x.(mem_ins) = non /\ memory_trace = memory_trace'))).
+    {
+      apply (exists_memory_trace' l memory_trace x); try tauto;
+      apply (last_action_trace_timestamp_biggest (l ++ [x]) l x); tauto.
+    }
+    inversion H13 as [memory_trace' H14]. clear H13.
+    destruct H14 as [H14 H_for_last_mem].
+    assert (constraints program rm_last_CPU_trace l memory_trace').
+    {
+      apply all_constraints.
+      apply H10.
+      apply H11.
+      apply H12.
+      apply H9.
+      inversion H14. subst.
+      apply H13.
+      inversion H14. subst.
+      apply H15.
+      apply public.
+    }
+    assert (exists (rm_first_CPU_trace'
+    rm_last_CPU_trace' : list CPU_state)
+    (first_CPU_state' last_CPU_state' : CPU_state),
+    rm_last_CPU_trace = first_CPU_state' :: rm_first_CPU_trace' /\
+    rm_last_CPU_trace = rm_last_CPU_trace' ++ [last_CPU_state']).
+    {
+      apply action_CPU_trace_len_cons in H9.
+      destruct rm_last_CPU_trace.
+      - discriminate.
+      - exists rm_last_CPU_trace.
+        specialize (cons_app_eq c rm_last_CPU_trace).
+        intros.
+        destruct H15. destruct H15.
+        exists x1, c, x0.
+        split.
+        + tauto.
+        + apply H15.
+    }
+    inversion H15 as [rm_first_CPU_trace' H16]. clear H15.
+    inversion H16 as [rm_last_CPU_trace' H17]. clear H16.
+    inversion H17 as [first_CPU_state' H18]. clear H17.
+    inversion H18 as [last_CPU_state' H19]. clear H18.
+    inversion H19 as [H20 H21]. clear H19.
+    apply (H program rm_last_CPU_trace rm_first_CPU_trace' rm_last_CPU_trace'
+    first_CPU_state' last_CPU_state' memory_trace') in H13; try tauto.
+    inversion H13 as [mem_list' H15]. clear H13.
+    inversion H15 as [first_mem' H13]. clear H15.
+    inversion H13 as [last_mem' H15]. clear H13.
+    exists (mem_list' ++ [last_mem']). exists first_mem'.
+    assert (exists last_mem, last_mem = (fun address0 =>
+      match x.(mem_ins) with
+      | write address value => if (Int256.eq address address0) then value else (last_mem' address0)
+      | _ => last_mem' address0
+      end
+    ) /\ (forall address : int256,
+    last_mem_prop last_mem memory_trace
+      address)).
+    { 
+      destruct H15; destruct H15.
+      exists (fun address0 =>
+        match x.(mem_ins) with
+        | write address value => if (Int256.eq address address0) then value else (last_mem' address0)
+        | _ => last_mem' address0
+        end
+      ).
+      intros.
+      inversion H14. clear H19 H22 action_trace0 memory_trace0.
+      pose proof (last_action_trace_timestamp_biggest (l ++ [x]) l x).
+      assert (Forall
+      (fun a : action_type =>
+       a.(timestamp) < x.(timestamp)) l).
+      {
+        assert (l ++ [x] = l ++ [x]). { tauto. }
+        apply (H19 H22 H4).
+      }
+      clear H19.
+      split; try tauto.
+      intro.
+      apply (construct_last_mem
+      memory_trace memory_trace' l 
+      x address last_mem' H7 H6 H18 H17 H22 H_for_last_mem).
+      tauto.
+    }
+    destruct H13 as [last_mem H13]. 
+    assert (eval_ins_list_single program
+    (combine_to_pc_state last_CPU_state' last_mem')
+    (combine_to_act_state_list [last_CPU_state']
+      [last_mem'] 
+      [x])
+    (combine_to_pc_state last_CPU_state last_mem)).
+    {
+      rewrite H21 in H5.
+      inversion H5.
+      inversion H16.
+      - symmetry in H23.
+        apply app_eq_nil in H23.
+        inversion H23.
+        discriminate.
+      - apply app_inj_tail in H19.
+        inversion H19. clear H19.
+        apply app_inj_tail in H25.
+        inversion H25. clear H25.
+        apply app_inj_tail in H22.
+        inversion H22. clear H22.
+        rewrite H27 in H23.
+        rewrite H26 in H23.
+        rewrite H28 in H23.
+        destruct H15.
+        destruct H22.
+        inversion H1. clear H30 H31 H32 H34 CPU_trace0 rm_first_CPU_trace0 first_CPU_state0.
+        rewrite H21 in H33.
+        inversion H33.
+        + symmetry in H31.
+          apply app_eq_unit in H31.
+          destruct H31.
+          {
+            destruct H30.
+            apply app_eq_nil in H30.
+            destruct H30.
+            discriminate.
+          }
+          {
+            destruct H30.
+            discriminate.
+          }
+        + assert (l1 ++ [x1; y0] = (l1 ++ [x1]) ++ [y0]). { rewrite <- app_assoc; tauto. }
+          rewrite H34 in H30.
+          apply app_inj_tail in H30.
+          destruct H30.
+          apply app_inj_tail in H30.
+          destruct H30.
+          rewrite H36, H35 in H31.
+          clear H32 H30 H36 H34 H35 H33 x1 y0 l1.
+          clear H26 H19 H25 H28 H24 H27 H18 l0 x0 y action0 l_action H17 H16 action_trace0 CPU_trace action_trace0.
+          inversion H23.
+          {
+            clear H24 H25 H26 state0 next_state action0.
+            unfold eval_constraint in H31.
+            rewrite H16 in H31.
+            assert (MLOAD_sem last_CPU_state'.(pc) (combine_to_pc_state last_CPU_state'
+            last_mem') (combine_to_act_state_list
+            [last_CPU_state'] [last_mem'] [x]) (combine_to_pc_state last_CPU_state
+            last_mem)).
+            {
+              inversion H31. clear H26 H27 x0 y.
+              inversion H25. clear H27 H25 offset value0.
+              assert (last_mem' address = value).
+              {
+                specialize (H29 address).
+                destruct H_for_last_mem; destruct H25.
+                - destruct H26 as [l1 [l2 H26]].
+                  destruct H26 as [H_pre H_now].
+                  inversion H14.
+                  apply (additional_property_to_for_new_read address value x memory_trace memory_trace' l1 l2 l last_mem' H7 H27 H26 H6 H4 H_pre H_now H17 H29).
+                - rewrite H25 in H17.
+                  discriminate.
+              }
+              apply mload_sem with (offset := address) (l := remaining_stack); try tauto.
+              {
+                assert (((combine_to_pc_state last_CPU_state' last_mem').(state)).(memory) address = value).
+                {
+                  unfold combine_to_pc_state.
+                  tauto.
+                }
+                rewrite H26.
+                unfold combine_to_pc_state.
+                tauto.
+              }
+              {
+                simpl.
+                destruct H13.
+                rewrite H13.
+                rewrite H17.
+                reflexivity.
+              }
+              {
+                simpl.
+                rewrite H25.
+                tauto.
+              }
+            }
+            assert (In (last_CPU_state'.(inst), last_CPU_state'.(pc)) (combine program
+            (seq 0 (Datatypes.length program)))).
+            {
+              inversion H11.
+              clear H27 program0.
+              rewrite Forall_forall in H25.
+              assert (In (last_CPU_state'.(inst), last_CPU_state'.(pc)) (map
+              (fun cpu_state : CPU_state =>
+               (cpu_state.(inst), cpu_state.(pc)))
+              rm_last_CPU_trace)).
+              {
+                rewrite H21.
+                rewrite map_app.
+                apply in_or_app.
+                right.
+                simpl.
+                left.
+                tauto.
+              }
+              apply (H25 (last_CPU_state'.(inst), last_CPU_state'.(pc)) H27).
+            }
+            constructor.
+            unfold fold_ins_sem.
+            assert (eval_ins (last_CPU_state'.(inst), last_CPU_state'.(pc)) (combine_to_pc_state last_CPU_state'
+            last_mem') (combine_to_act_state_list
+            [last_CPU_state'] [last_mem'] [x]) (combine_to_pc_state last_CPU_state
+            last_mem)).
+            {
+              unfold eval_ins.
+              rewrite H16.
+              tauto.
+            }
+            apply (in_property (ins * nat) 
+            pc_state (list act_state) pc_state (last_CPU_state'.(inst), last_CPU_state'.(pc))
+            (combine program (seq 0 (Datatypes.length program)))
+            eval_ins
+            (combine_to_pc_state last_CPU_state' last_mem')
+            (combine_to_act_state_list [last_CPU_state'] [last_mem'] [x])
+            (combine_to_pc_state last_CPU_state last_mem)
+            ); tauto.
+          }
+          {
+            clear H24 H25 H19 state0 next_state action0.
+            unfold eval_constraint in H31.
+            rewrite H16 in H31.
+            assert (MSTORE_sem last_CPU_state'.(pc) (combine_to_pc_state last_CPU_state'
+            last_mem') (combine_to_act_state_list
+            [last_CPU_state'] [last_mem'] [x]) (combine_to_pc_state last_CPU_state
+            last_mem)).
+            {
+              inversion H31. clear H25 H26 x0 y.
+              rewrite H18 in H24.
+              inversion H24.
+              rewrite H28 in H18.
+              clear H24 H26 H27 H28 offset value0.
+              apply mstore_sem with (offset := address) (v := value); try tauto.
+              destruct H13.
+              rewrite H13.
+              rewrite H17.
+              simpl.
+              unfold update_memory.
+              apply functional_extensionality.
+              intros address0.
+              destruct (Int256.eq_dec address address0).
+              - rewrite e. reflexivity.
+              - pose proof n as n'.
+                apply not_eq_sym in n'.
+                apply Int256.eq_false in n.
+                apply Int256.eq_false in n'.
+                rewrite n, n'.
+                reflexivity.
+            }
+            assert (In (last_CPU_state'.(inst), last_CPU_state'.(pc)) (combine program
+            (seq 0 (Datatypes.length program)))).
+            {
+              inversion H11.
+              clear H26 program0.
+              rewrite Forall_forall in H24.
+              assert (In (last_CPU_state'.(inst), last_CPU_state'.(pc)) (map
+              (fun cpu_state : CPU_state =>
+               (cpu_state.(inst), cpu_state.(pc)))
+              rm_last_CPU_trace)).
+              {
+                rewrite H21.
+                rewrite map_app.
+                apply in_or_app.
+                right.
+                simpl.
+                left.
+                tauto.
+              }
+              apply (H24 (last_CPU_state'.(inst), last_CPU_state'.(pc)) H26).
+            }
+            constructor.
+            unfold fold_ins_sem.
+            assert (eval_ins (last_CPU_state'.(inst), last_CPU_state'.(pc)) (combine_to_pc_state last_CPU_state'
+            last_mem') (combine_to_act_state_list
+            [last_CPU_state'] [last_mem'] [x]) (combine_to_pc_state last_CPU_state
+            last_mem)).
+            {
+              unfold eval_ins.
+              rewrite H16.
+              tauto.
+            }
+            apply (in_property (ins * nat) 
+            pc_state (list act_state) pc_state (last_CPU_state'.(inst), last_CPU_state'.(pc))
+            (combine program (seq 0 (Datatypes.length program)))
+            eval_ins
+            (combine_to_pc_state last_CPU_state' last_mem')
+            (combine_to_act_state_list [last_CPU_state'] [last_mem'] [x])
+            (combine_to_pc_state last_CPU_state last_mem)
+            ); tauto.
+          }
+          {
+            clear H24 H25 H19 state0 next_state action0.
+            unfold eval_constraint in H31.
+            destruct last_CPU_state'.(inst) eqn: H_ins.
+            - assert (JUMPI_sem last_CPU_state'.(pc) (combine_to_pc_state last_CPU_state'
+              last_mem') (combine_to_act_state_list
+              [last_CPU_state'] [last_mem'] [x]) (combine_to_pc_state last_CPU_state
+              last_mem)).
+              {
+                inversion H31.
+                apply jumpi_sem with (dest := dest) (cond := cond); try tauto.
+                simpl.
+                destruct H13.
+                rewrite H13.
+                rewrite H18.
+                reflexivity.
+              }
+              assert (In (last_CPU_state'.(inst), last_CPU_state'.(pc)) (combine program
+              (seq 0 (Datatypes.length program)))).
+              {
+                inversion H11.
+                clear H26 program0.
+                rewrite Forall_forall in H24.
+                assert (In (last_CPU_state'.(inst), last_CPU_state'.(pc)) (map
+                (fun cpu_state : CPU_state =>
+                (cpu_state.(inst), cpu_state.(pc)))
+                rm_last_CPU_trace)).
+                {
+                  rewrite H21.
+                  rewrite map_app.
+                  apply in_or_app.
+                  right.
+                  simpl.
+                  left.
+                  tauto.
+                }
+                apply (H24 (last_CPU_state'.(inst), last_CPU_state'.(pc)) H26).
+              }
+              constructor.
+              unfold fold_ins_sem.
+              assert (eval_ins (last_CPU_state'.(inst), last_CPU_state'.(pc)) (combine_to_pc_state last_CPU_state'
+              last_mem') (combine_to_act_state_list
+              [last_CPU_state'] [last_mem'] [x]) (combine_to_pc_state last_CPU_state
+              last_mem)).
+              {
+                unfold eval_ins.
+                rewrite H_ins.
+                tauto.
+              }
+              apply (in_property (ins * nat) 
+              pc_state (list act_state) pc_state (last_CPU_state'.(inst), last_CPU_state'.(pc))
+              (combine program (seq 0 (Datatypes.length program)))
+              eval_ins
+              (combine_to_pc_state last_CPU_state' last_mem')
+              (combine_to_act_state_list [last_CPU_state'] [last_mem'] [x])
+              (combine_to_pc_state last_CPU_state last_mem)
+              ); tauto.
+            - assert (JUMP_sem last_CPU_state'.(pc) (combine_to_pc_state last_CPU_state'
+              last_mem') (combine_to_act_state_list
+              [last_CPU_state'] [last_mem'] [x]) (combine_to_pc_state last_CPU_state
+              last_mem)).
+              {
+                inversion H31.
+                apply jump_sem with (v := v); try tauto.
+                simpl.
+                destruct H13.
+                rewrite H13.
+                rewrite H18.
+                reflexivity.
+              }
+              assert (In (last_CPU_state'.(inst), last_CPU_state'.(pc)) (combine program
+              (seq 0 (Datatypes.length program)))).
+              {
+                inversion H11.
+                clear H26 program0.
+                rewrite Forall_forall in H24.
+                assert (In (last_CPU_state'.(inst), last_CPU_state'.(pc)) (map
+                (fun cpu_state : CPU_state =>
+                (cpu_state.(inst), cpu_state.(pc)))
+                rm_last_CPU_trace)).
+                {
+                  rewrite H21.
+                  rewrite map_app.
+                  apply in_or_app.
+                  right.
+                  simpl.
+                  left.
+                  tauto.
+                }
+                apply (H24 (last_CPU_state'.(inst), last_CPU_state'.(pc)) H26).
+              }
+              constructor.
+              unfold fold_ins_sem.
+              assert (eval_ins (last_CPU_state'.(inst), last_CPU_state'.(pc)) (combine_to_pc_state last_CPU_state'
+              last_mem') (combine_to_act_state_list
+              [last_CPU_state'] [last_mem'] [x]) (combine_to_pc_state last_CPU_state
+              last_mem)).
+              {
+                unfold eval_ins.
+                rewrite H_ins.
+                tauto.
+              }
+              apply (in_property (ins * nat) 
+              pc_state (list act_state) pc_state (last_CPU_state'.(inst), last_CPU_state'.(pc))
+              (combine program (seq 0 (Datatypes.length program)))
+              eval_ins
+              (combine_to_pc_state last_CPU_state' last_mem')
+              (combine_to_act_state_list [last_CPU_state'] [last_mem'] [x])
+              (combine_to_pc_state last_CPU_state last_mem)
+              ); tauto.
+            - assert (POP_sem last_CPU_state'.(pc) (combine_to_pc_state last_CPU_state'
+              last_mem') (combine_to_act_state_list
+              [last_CPU_state'] [last_mem'] [x]) (combine_to_pc_state last_CPU_state
+              last_mem)).
+              {
+                inversion H31.
+                apply pop_sem with (v := v); try tauto.
+                simpl.
+                destruct H13.
+                rewrite H13.
+                rewrite H18.
+                reflexivity.
+              }
+              assert (In (last_CPU_state'.(inst), last_CPU_state'.(pc)) (combine program
+              (seq 0 (Datatypes.length program)))).
+              {
+                inversion H11.
+                clear H26 program0.
+                rewrite Forall_forall in H24.
+                assert (In (last_CPU_state'.(inst), last_CPU_state'.(pc)) (map
+                (fun cpu_state : CPU_state =>
+                (cpu_state.(inst), cpu_state.(pc)))
+                rm_last_CPU_trace)).
+                {
+                  rewrite H21.
+                  rewrite map_app.
+                  apply in_or_app.
+                  right.
+                  simpl.
+                  left.
+                  tauto.
+                }
+                apply (H24 (last_CPU_state'.(inst), last_CPU_state'.(pc)) H26).
+              }
+              constructor.
+              unfold fold_ins_sem.
+              assert (eval_ins (last_CPU_state'.(inst), last_CPU_state'.(pc)) (combine_to_pc_state last_CPU_state'
+              last_mem') (combine_to_act_state_list
+              [last_CPU_state'] [last_mem'] [x]) (combine_to_pc_state last_CPU_state
+              last_mem)).
+              {
+                unfold eval_ins.
+                rewrite H_ins.
+                tauto.
+              }
+              apply (in_property (ins * nat) 
+              pc_state (list act_state) pc_state (last_CPU_state'.(inst), last_CPU_state'.(pc))
+              (combine program (seq 0 (Datatypes.length program)))
+              eval_ins
+              (combine_to_pc_state last_CPU_state' last_mem')
+              (combine_to_act_state_list [last_CPU_state'] [last_mem'] [x])
+              (combine_to_pc_state last_CPU_state last_mem)
+              ); tauto.
+            - assert (ADD_sem last_CPU_state'.(pc) (combine_to_pc_state last_CPU_state'
+              last_mem') (combine_to_act_state_list
+              [last_CPU_state'] [last_mem'] [x]) (combine_to_pc_state last_CPU_state
+              last_mem)).
+              {
+                inversion H31.
+                apply add_sem with (v1 := v1) (v2 := v2) (l := l0); try simpl; try tauto.
+                destruct H13.
+                rewrite H13.
+                rewrite H18.
+                reflexivity.
+              }
+              assert (In (last_CPU_state'.(inst), last_CPU_state'.(pc)) (combine program
+              (seq 0 (Datatypes.length program)))).
+              {
+                inversion H11.
+                clear H26 program0.
+                rewrite Forall_forall in H24.
+                assert (In (last_CPU_state'.(inst), last_CPU_state'.(pc)) (map
+                (fun cpu_state : CPU_state =>
+                (cpu_state.(inst), cpu_state.(pc)))
+                rm_last_CPU_trace)).
+                {
+                  rewrite H21.
+                  rewrite map_app.
+                  apply in_or_app.
+                  right.
+                  simpl.
+                  left.
+                  tauto.
+                }
+                apply (H24 (last_CPU_state'.(inst), last_CPU_state'.(pc)) H26).
+              }
+              constructor.
+              unfold fold_ins_sem.
+              assert (eval_ins (last_CPU_state'.(inst), last_CPU_state'.(pc)) (combine_to_pc_state last_CPU_state'
+              last_mem') (combine_to_act_state_list
+              [last_CPU_state'] [last_mem'] [x]) (combine_to_pc_state last_CPU_state
+              last_mem)).
+              {
+                unfold eval_ins.
+                rewrite H_ins.
+                tauto.
+              }
+              apply (in_property (ins * nat) 
+              pc_state (list act_state) pc_state (last_CPU_state'.(inst), last_CPU_state'.(pc))
+              (combine program (seq 0 (Datatypes.length program)))
+              eval_ins
+              (combine_to_pc_state last_CPU_state' last_mem')
+              (combine_to_act_state_list [last_CPU_state'] [last_mem'] [x])
+              (combine_to_pc_state last_CPU_state last_mem)
+              ); tauto.
+            - assert (MUL_sem last_CPU_state'.(pc) (combine_to_pc_state last_CPU_state'
+              last_mem') (combine_to_act_state_list
+              [last_CPU_state'] [last_mem'] [x]) (combine_to_pc_state last_CPU_state
+              last_mem)).
+              {
+                inversion H31.
+                apply mul_sem with (v1 := v1) (v2 := v2) (l := l0); try simpl; try tauto.
+                destruct H13.
+                rewrite H13.
+                rewrite H18.
+                reflexivity.
+              }
+              assert (In (last_CPU_state'.(inst), last_CPU_state'.(pc)) (combine program
+              (seq 0 (Datatypes.length program)))).
+              {
+                inversion H11.
+                clear H26 program0.
+                rewrite Forall_forall in H24.
+                assert (In (last_CPU_state'.(inst), last_CPU_state'.(pc)) (map
+                (fun cpu_state : CPU_state =>
+                (cpu_state.(inst), cpu_state.(pc)))
+                rm_last_CPU_trace)).
+                {
+                  rewrite H21.
+                  rewrite map_app.
+                  apply in_or_app.
+                  right.
+                  simpl.
+                  left.
+                  tauto.
+                }
+                apply (H24 (last_CPU_state'.(inst), last_CPU_state'.(pc)) H26).
+              }
+              constructor.
+              unfold fold_ins_sem.
+              assert (eval_ins (last_CPU_state'.(inst), last_CPU_state'.(pc)) (combine_to_pc_state last_CPU_state'
+              last_mem') (combine_to_act_state_list
+              [last_CPU_state'] [last_mem'] [x]) (combine_to_pc_state last_CPU_state
+              last_mem)).
+              {
+                unfold eval_ins.
+                rewrite H_ins.
+                tauto.
+              }
+              apply (in_property (ins * nat) 
+              pc_state (list act_state) pc_state (last_CPU_state'.(inst), last_CPU_state'.(pc))
+              (combine program (seq 0 (Datatypes.length program)))
+              eval_ins
+              (combine_to_pc_state last_CPU_state' last_mem')
+              (combine_to_act_state_list [last_CPU_state'] [last_mem'] [x])
+              (combine_to_pc_state last_CPU_state last_mem)
+              ); tauto.
+            - assert (SUB_sem last_CPU_state'.(pc) (combine_to_pc_state last_CPU_state'
+              last_mem') (combine_to_act_state_list
+              [last_CPU_state'] [last_mem'] [x]) (combine_to_pc_state last_CPU_state
+              last_mem)).
+              {
+                inversion H31.
+                apply sub_sem with (v1 := v1) (v2 := v2) (l := l0); try simpl; try tauto.
+                destruct H13.
+                rewrite H13.
+                rewrite H18.
+                reflexivity.
+              }
+              assert (In (last_CPU_state'.(inst), last_CPU_state'.(pc)) (combine program
+              (seq 0 (Datatypes.length program)))).
+              {
+                inversion H11.
+                clear H26 program0.
+                rewrite Forall_forall in H24.
+                assert (In (last_CPU_state'.(inst), last_CPU_state'.(pc)) (map
+                (fun cpu_state : CPU_state =>
+                (cpu_state.(inst), cpu_state.(pc)))
+                rm_last_CPU_trace)).
+                {
+                  rewrite H21.
+                  rewrite map_app.
+                  apply in_or_app.
+                  right.
+                  simpl.
+                  left.
+                  tauto.
+                }
+                apply (H24 (last_CPU_state'.(inst), last_CPU_state'.(pc)) H26).
+              }
+              constructor.
+              unfold fold_ins_sem.
+              assert (eval_ins (last_CPU_state'.(inst), last_CPU_state'.(pc)) (combine_to_pc_state last_CPU_state'
+              last_mem') (combine_to_act_state_list
+              [last_CPU_state'] [last_mem'] [x]) (combine_to_pc_state last_CPU_state
+              last_mem)).
+              {
+                unfold eval_ins.
+                rewrite H_ins.
+                tauto.
+              }
+              apply (in_property (ins * nat) 
+              pc_state (list act_state) pc_state (last_CPU_state'.(inst), last_CPU_state'.(pc))
+              (combine program (seq 0 (Datatypes.length program)))
+              eval_ins
+              (combine_to_pc_state last_CPU_state' last_mem')
+              (combine_to_act_state_list [last_CPU_state'] [last_mem'] [x])
+              (combine_to_pc_state last_CPU_state last_mem)
+              ); tauto.
+            - congruence.
+            - congruence.
+            - assert (PUSH32_sem v last_CPU_state'.(pc) (combine_to_pc_state last_CPU_state'
+              last_mem') (combine_to_act_state_list
+              [last_CPU_state'] [last_mem'] [x]) (combine_to_pc_state last_CPU_state
+              last_mem)).
+              {
+                inversion H31.
+                apply push32_sem; try simpl; try tauto.
+                destruct H13.
+                rewrite H13.
+                rewrite H18.
+                reflexivity.
+              }
+              assert (In (last_CPU_state'.(inst), last_CPU_state'.(pc)) (combine program
+              (seq 0 (Datatypes.length program)))).
+              {
+                inversion H11.
+                clear H26 program0.
+                rewrite Forall_forall in H24.
+                assert (In (last_CPU_state'.(inst), last_CPU_state'.(pc)) (map
+                (fun cpu_state : CPU_state =>
+                (cpu_state.(inst), cpu_state.(pc)))
+                rm_last_CPU_trace)).
+                {
+                  rewrite H21.
+                  rewrite map_app.
+                  apply in_or_app.
+                  right.
+                  simpl.
+                  left.
+                  tauto.
+                }
+                apply (H24 (last_CPU_state'.(inst), last_CPU_state'.(pc)) H26).
+              }
+              constructor.
+              unfold fold_ins_sem.
+              assert (eval_ins (last_CPU_state'.(inst), last_CPU_state'.(pc)) (combine_to_pc_state last_CPU_state'
+              last_mem') (combine_to_act_state_list
+              [last_CPU_state'] [last_mem'] [x]) (combine_to_pc_state last_CPU_state
+              last_mem)).
+              {
+                unfold eval_ins.
+                rewrite H_ins.
+                tauto.
+              }
+              apply (in_property (ins * nat) 
+              pc_state (list act_state) pc_state (last_CPU_state'.(inst), last_CPU_state'.(pc))
+              (combine program (seq 0 (Datatypes.length program)))
+              eval_ins
+              (combine_to_pc_state last_CPU_state' last_mem')
+              (combine_to_act_state_list [last_CPU_state'] [last_mem'] [x])
+              (combine_to_pc_state last_CPU_state last_mem)
+              ); tauto.
+          }
+    }
+    destruct H15.
+    destruct H17.
+    exists last_mem.
+    assert (first_CPU_state' = first_CPU_state).
+    {
+      rewrite H20 in H2. Search app.
+      rewrite <- app_comm_cons in H2.
+      inversion H2.
+      tauto.
+    }
+    rewrite H19 in H17.
+    inversion H17.
+    split.
+    {
+      rewrite ! last_length.
+      lia.
+    }
+    clear H19 H27 H28 H29 H30 l0 x0 y z.
+    apply and_comm.
+    split; try tauto.
+    clear H18 H13.
+    apply sigma; try auto.
+    {
+      clear H22 H23 H24 H26.
+      inversion H4.
+      - symmetry in H18; apply app_eq_nil in H18; inversion H18; discriminate.
+      - symmetry in H13; apply app_eq_unit in H13.
+        inversion H13.
+        + inversion H19.
+          apply length_zero_iff_nil in H22.
+          rewrite H22 in H15.
+          apply action_CPU_trace_len_cons in H9.
+          rewrite H22 in H9.
+          apply length_one_iff_single in H9.
+          inversion H9.
+          rewrite H24.
+          apply length_zero_iff_nil in H15.
+          rewrite H15.
+          simpl.
+          apply ActionListSingle.
+          simpl.
+          apply H18.
+        + inversion H19.
+          discriminate.
+      - rewrite H21.
+        apply app_inj_tail in H13.
+        inversion H13.
+        rewrite <- H22 in H25.
+        apply action_CPU_trace_len_cons in H9.
+        rewrite H21 in H9.
+        rewrite last_length in H9.
+        apply eq_add_S in H9.
+        rewrite <- H22 in H9.
+        destruct rm_last_CPU_trace'.
+        + simpl in H9.
+          symmetry in H9.
+          apply length_zero_iff_nil in H9.
+          apply app_eq_nil in H9.
+          inversion H9.
+          discriminate.
+        + destruct mem_list'.
+          * rewrite <- H22 in H15.
+            symmetry in H15.
+            simpl in H15.
+            apply length_zero_iff_nil in H15.
+            apply app_eq_nil in H15.
+            inversion H15.
+            discriminate.
+          * specialize (cons_app_eq c rm_last_CPU_trace').
+            intros. destruct H24. destruct H24.
+            specialize (cons_app_eq i mem_list').
+            intros. destruct H26. destruct H26.
+            rewrite H24, H26 in H25.
+            rewrite H24, H26.
+            assert (Datatypes.length (x2 ++ [x1]) =
+                Datatypes.length (x4 ++ [x3])).
+            {
+              rewrite H22 in H9.
+              rewrite <- H9 in H15.
+              rewrite <- H24. rewrite <- H26.
+              rewrite H15.
+              tauto.
+            }
+            assert (Datatypes.length
+            (combine (x2 ++ [x1]) (x4 ++ [x3])) =
+            Datatypes.length (l0 ++ [x0])).
+            {
+              apply len_combine in H27.
+              rewrite <- H27.
+              rewrite <- H26.
+              rewrite H22.
+              apply H15.
+            }
+            assert (Datatypes.length
+            (combine [last_CPU_state'] [last_mem']) =
+            Datatypes.length [y]).
+            {
+              assert (length [last_CPU_state'] = length [last_mem']).
+              { tauto. }
+              apply len_combine in H29.
+              rewrite <- H29.
+              tauto.
+            }
+            assert (Datatypes.length x2 = Datatypes.length x4).
+            {
+              rewrite ! app_length in H27.
+              simpl in H27.
+              lia.
+            }
+            assert (Datatypes.length [x1] = Datatypes.length [x3]).
+            {
+              tauto.
+            }
+            assert (Datatypes.length (combine x2 x4) =
+            Datatypes.length l0).
+            {
+              rewrite combine_app in H28; try tauto.
+              rewrite ! app_length in H28.
+              apply len_combine in H31.
+              rewrite <- H31 in H28.
+              simpl in H28.
+              lia.
+            }
+            assert (Datatypes.length (combine [x1] [x3]) =
+            Datatypes.length [x3]).
+            {
+              apply len_combine in H31.
+              rewrite <- H31.
+              tauto.
+            }
+            unfold combine_to_act_state_list.
+            rewrite combine_app; try tauto.
+            rewrite combine_app; try tauto.
+            rewrite map_app; try tauto.
+            rewrite combine_app; try tauto.
+            rewrite combine_app; try tauto.
+            rewrite map_app.
+            apply ActionListCons; try tauto.
+            rewrite <- H22 in H17.
+            rewrite H24 in H17.
+            rewrite H26 in H17.
+            unfold combine_to_act_state_list in H17.
+            rewrite combine_app in H17; try tauto.
+            rewrite combine_app in H17; try tauto.
+            rewrite map_app in H17.
+            simpl in H17.
+            inversion H17. subst.
+            apply H37.
+      (* Increasing_timestamp *)
+    }
+    {
+      clear H22 H23 H24 H25.
+      (* eval_ins_list_single *)
+      rewrite H21.
+      pose proof (rt_trans_n1 (eval_ins_list_single program)).
+      assert ((combine_to_pc_state first_CPU_state first_mem',
+      combine_to_act_state_list (rm_last_CPU_trace' ++ [last_CPU_state'])
+      (mem_list' ++ [last_mem']) (l ++ [x]),
+      combine_to_pc_state last_CPU_state last_mem)
+      ∈ clos_refl_trans (eval_ins_list_single program)
+      ∘ eval_ins_list_single program).
+      {
+        simpl.
+        exists (combine_to_pc_state last_CPU_state' last_mem').
+        exists (combine_to_act_state_list rm_last_CPU_trace' mem_list' l).
+        exists (combine_to_act_state_list [last_CPU_state'] [last_mem'] [x]).
+        split.
+        - assert (combine_to_act_state_list rm_last_CPU_trace' mem_list' l ++
+          combine_to_act_state_list [last_CPU_state'] [last_mem'] [x] =
+          combine_to_act_state_list (rm_last_CPU_trace' ++ [last_CPU_state'])
+          (mem_list' ++ [last_mem']) (l ++ [x])).
+          {
+            unfold combine_to_act_state_list.
+            unfold combine_to_act_state.
+            rewrite <- map_app.
+            assert (combine (combine rm_last_CPU_trace' mem_list') l ++
+            combine (combine [last_CPU_state'] [last_mem']) [x] =
+            combine (combine (rm_last_CPU_trace' ++ [last_CPU_state']) (mem_list' ++ [last_mem'])) (l ++ [x])).
+            {
+              (* combine property, correct only when
+              rm_last_CPU_trace, mem_list and action_trace have the same length,
+              which need a lemma to prove it *)
+              assert (length rm_last_CPU_trace' = length mem_list').
+              { 
+                assert (length rm_last_CPU_trace' = length l).
+                {
+                  assert (length rm_last_CPU_trace = S (length l)).
+                  {
+                    apply action_CPU_trace_len_cons.
+                    apply H9.
+                  }
+                  rewrite H21 in H18.
+                  simpl in H18.
+                  rewrite last_length in H18.
+                  injection H18.
+                  intros. apply H19.
+                }
+                rewrite H15.  apply H18.
+              }
+              rewrite ! combine_app; try tauto.
+              apply len_combine in H18.
+              rewrite <- H18.
+              tauto.
+            }
+            rewrite H18.
+            reflexivity.
+          }
+          apply H18.
+        - split.
+          + simpl.
+            inversion H17. apply H24.
+          + apply H16.
+      }
+      apply H13 in H18. apply H18.
+    }
+Qed.
